cambios en reunion 17/10 2

src/Especificacion.dfy
@@ -1,3 +1,5 @@
+include "ContainersOps.dfy"
+include "Math.dfy"
 //A nivel de especificación tenemos estos datatype
 
 datatype ItemData = ItemData(weight: real, value: real) {
@@ -6,13 +8,48 @@ datatype ItemData = ItemData(weight: real, value: real) {
   }
 }
 
-datatype InputData = InputData(itemsD: seq<ItemData>, maxWeight: real)
+datatype InputData = InputData(items: seq<ItemData>, maxWeight: real) {
+  ghost predicate Valid() {
+    (forall i | 0 <= i < |items| :: items[i].Valid()) &&
+    maxWeight >= 0.0
+  }
+}
 
-datatype SolutionData = SolutionData(itemsAssign: seq<bool>, totalWeight: real, totalValue: real, k: int) {
+datatype SolutionData = SolutionData(itemsAssign: seq<bool>, k: nat) {
+
+  ghost function TotalWeight(items: seq<ItemData>): real
+    requires k <= |items|
+    requires k <= |itemsAssign|
+  {
+    var objSelected: seq<ItemData> := selectSeq(items, itemsAssign, 0, k);
+    var numSelected: nat := |objSelected|;
+    var weightsSelected: seq<real> := mapSeq(objSelected, (obj: ItemData) => obj.weight, 0, numSelected);
+    sum_real(weightsSelected, 0, numSelected)
+  }
+
+  ghost function SolutionValue(items: seq<ItemData>): (o: real)
+	requires k <= |items|
+	requires k <= |itemsAssign|
+  {
+	var objSelected: seq<ItemData> := selectSeq(items, itemsAssign, 0, k);
+	var numSelected: nat := |objSelected|;
+	var valuesSelected: seq<real> := mapSeq(objSelected, (obj: ItemData) => obj.value, 0, numSelected);
+	sum_real(valuesSelected, 0, numSelected)
+  }
+
+  ghost predicate OptimalSolution(items: seq<ItemData>, itemEndIdx: nat, availableWeight: real, itemsAssign: seq<bool>)
+	requires ValidInstance(items,availableWeight)
+	requires itemEndIdx <= |items|
+	requires itemEndIdx <= |itemsAssign|
+	requires ValidSolution(items, itemEndIdx, availableWeight, itemsAssign)
+{
+	forall otherSolution: seq<bool> | itemEndIdx <= |otherSolution| && ValidSolution(items, itemEndIdx, availableWeight, otherSolution) :: SolutionValue(items, itemEndIdx, otherSolution) <= SolutionValue(items, itemEndIdx, itemsAssign)
+}
+
   ghost predicate Valid(input: InputData){
     0 <= k <= |itemsAssign| &&
-    |itemsAssign| == |input.itemsD|
-    && totalWeight <= input.maxWeight    
+    |itemsAssign| == |input.items|
+    && TotalWeight(input.items) <= input.maxWeight    
   }
 
 }
