src/Solution.dfy
@@ -1,24 +1,31 @@
 include "Item.dfy"
+include "Especificacion.dfy"
 
 class Solution {
   var itemsAssign: array<bool> //objetos seleccionados (si o no)
   var totalValue: real
   var totalWeight: real
-  var k: int
+  var k: nat
 
-  constructor(itemsAssign: array<bool>, totalV: real, totalW: real, k': int) {
+  constructor(itemsAssign: array<bool>, totalV: real, totalW: real, k': nat) {
     this.itemsAssign := itemsAssign;
     this.totalValue := totalV;
     this.totalWeight := totalW;
     this.k := k';
   }
 
-  predicate Valid (items: array<Item> , maxWeight: real)
-    reads this
+  ghost predicate Valid (input : InputData)
+    reads this, itemsAssign
   {
-    0 <= this.k <= this.itemsAssign.Length &&
-    this.itemsAssign.Length == items.Length &&
-    this.totalWeight <= maxWeight
+    && Model().Valid(input) 
+    && Model().TotalWeight(input.items) == totalWeight
+    && Model().SolutionValue(input.items) == totalValue
+  }
+
+  ghost function Model() : SolutionData 
+  reads this, itemsAssign
+  {
+    SolutionData(itemsAssign[..], k)
   }
 
 
